<?xml version="1.0" encoding="UTF-8"?>

<section xml:id="sec_fourth-intro" xmlns:xi="http://www.w3.org/2001/XInclude">
  <title>Simple Harmonic Motion</title>

  <introduction>
    <p>
     <idx>shm</idx> A motion of a particle in which it repeats its position after a fixed 
     interval of time is known as <em>periodic motion</em>. A periodic motion in which a restoring 
     force acting on a particle is proportional to its displacement is known as <em>simple harmonic motion</em> (SHM). 
     A planet orbits around the sun, bouncing ball, vibrating tuning fork, oscillation of pendulum 
     are all periodic motion but only vibrating tuning fork, oscillation of pendulum, to and fro motion 
     of spring-mass system are simple harmonic motion. The motion of planet around the sun, 
     motion of a bouncing ball are periodic but not simple harmonic as their motion is not 
     repetitive towards or from the mean position. 
    </p>
    <p>
      When a wave propagates through a medium it displaces the medium particles at rest from their mean 
      (equilibrium) positions. Since the material of a medium has elastic property, surface tension, 
      and has experienced the gravity the particles start experiencing a restoring to force which wants 
      to bring them to their equilibrium position. According to Hook's law the restoring force is directly 
      proportional to the displacement of the particle from its mean position and directed along the mean 
      position, i.e., 
      <me>
        F\propto y.
      </me>
      <me>
        \text{or,}\quad F = -ky
      </me>
      -ve sign indicates that the force F is opposite to the displacement y and k is called an <em>elastic constant</em> 
      (or force constant) of the material of the medium. 
      <me>
        \text{or,}\quad m a = -ky
      </me>
      where m is the mass of a oscillating particle. 
      <me>
        \text{or,}\quad a = \frac{\,d^{2}y}{\,dt^{2}}= -\frac{k}{m}y =-\omega^{2}y
      </me>
      <me>
        \text{or,}\quad \frac{\,d^{2}y}{\,dt^{2}}+\omega^{2}y=0
      </me>
      which is a differential form of SHM, and 
      <me>
        \omega = \sqrt{\frac{k}{m}} =  2\pi f
      </me>
       is an angular frequency and  <m>f = \frac{1}{T}</m>.
       <me>
        \text{or,}\quad a=\frac{\,dv}{\,dt} = -\omega^{2}y
       </me>
       <me>
        \text{or,}\quad \frac{\,dv}{\,dx}\frac{\,dx}{\,dt} = -\omega^{2}y
       </me>
       <me>
        \text{or,}\quad v\frac{\,dv}{\,dx}= -\omega^{2}y
       </me>
       <me>
        \text{or,}\quad \int\limits_{v_{o}}^{v} v \,dv = -\omega^{2}\int\limits_{y_{o}}^{y} y \,dy
       </me>
       <me>
        \text{or,}\quad \left.\frac{v^{2}}{2}\right\vert_{v_{o}}^{v} = -\omega^{2}\left.\frac{y^{2}}{2}\right\vert_{y_{o}}^{y}
       </me>
       <me>
        \text{or,}\quad  v^{2}-v_{o}^{2}= -\omega^{2}\left(y^{2}-y_{o}^{2}\right) 
       </me>
       <me>
        \text{or,}\quad  v^{2}= \omega^{2}\left(\frac{v_{o}^{2}}{\omega^{2}}+y_{o}^{2}-y^{2}\right)=\omega^{2}\left(A^{2} - y^{2}\right) 
       </me>
      <men xml:id="eqn-shm1">
        \text{or,}\quad v = \omega\sqrt{\left(A^{2}-y^{2}\right)} 
      </men>
      where 
      <me>
        A=\sqrt{\frac{v_{o}^{2}}{\omega^{2}}+y_{o}^{2}},
      </me>
      the amplitude or a maximum displacement of the particle. 
      <me>
        \text{or,}\quad v = \frac{\,dy}{\,dt}= \omega\sqrt{\left(A^{2}-y^{2}\right)}
      </me>
      <me>
        \text{or,}\quad  \frac{\,dy}{\sqrt{\left(A^{2}-y^{2}\right)}}= \omega\,dt
      </me>
      <men xml:id="eqn-shm2">
        \text{or,}\quad  \int\limits_{y_{o}}^{y}\frac{\,dy}{\sqrt{\left(A^{2}-y^{2}\right)}}= \omega \int\limits_{0}^{t}\,dt = \omega t 
      </men>
       To solve eqn. <xref ref="eqn-shm2"/>, consider 
       <me>
        \mathscr{I}= \int\frac{\,dy}{\sqrt{\left(A^{2}-y^{2}\right)}}
       </me>
          </p>
          <figure xml:id="rtangtrig">
            <caption></caption>
            <image source="rtangtrig.png" width="30%"/>
        </figure>
          <p>
            Now consider a right angled triangle as shown in <xref ref="rtangtrig"/>, 
             where  
             <me>
              \sin\theta = \frac{y}{A}
             </me>
             <me>
              \text{or,}\quad y=A \sin\theta
             </me>
             <me>
              \therefore \quad\,dy = A\cos\theta\,d\theta
             </me>
             <me>
              \text{or,}\quad  \mathscr{I} = \int\frac{A\cos\theta\,d\theta}{A\cos\theta} = \int\,d\theta = \theta = \sin^{-1}\frac{y}{A}
             </me>
             Hence from eqn. <xref ref="eqn-shm2"/>, we have - 
             <me>
              \left.\sin^{-1}\frac{y}{A}\right\vert_{y_{o}}^{y}=\omega t 
             </me>
             <me>
              \text{or,}\quad \sin^{-1}\frac{y}{A}-\sin^{-1}\frac{y_{o}}{A}=\omega t
             </me>
             <me>
              \text{or,}\quad \sin^{-1}\frac{y}{A} =\omega t+\sin^{-1}\frac{y_{o}}{A} = \omega t+\phi_{o} 
             </me>
             
             <men xml:id="eqn-shm3">
              \text{or,}\quad y = A\sin \left(\omega t+\phi_{o}\right)  
             </men>
                 </p>
                 <figure xml:id="rfc">
                  <caption></caption>
                  <sidebyside widths="30% 30%">
                       <figure xml:id="rfca">
                        <caption></caption>
                        <image source="rfca.png"/>
                    </figure>
                    <figure xml:id="rfcb">
                      <caption></caption>
                      <image source="rfcb.png"/>
                  </figure>
                  </sidebyside>
                </figure>
                 <p>
                  This is the solution for a differential form of SHM or also called an equation of SHM. 
                  Where  (<m>\omega t+\phi_{o}</m>) is called phase or phase angle of the particle. 
                  At t = 0, the particle position can be described by  <m>\phi_{o},</m>  an initial phase, 
                  or phase constant, or epoch of the particle. The phase angle is the angle swept out 
                  by a radial vector OP, the foot of a particle at time t on a reference circle as shown in <xref ref="rfc"/>.
                 </p>
                 <p>
                  The equation of SHM can be represented equivalently by 
                  <me>
                    y=A \cos(\omega t\pm \phi_{o})
                  </me>
                  <me>
                    \text{or,}\quad y = A\sin \left(\omega t\pm \phi_{o}\right)
                  </me>
                  The value of <m>\phi_{o} </m> depends upon the time from which it is counted. 
                  Let us consider the reference circle <xref ref="rfc"/> and time is counted from the point 
                  S above the mean position, then phase angle of the particle is 
                  <me>
                    \left(\omega t + \phi_{o}\right), 
                  </me>
                    if time is counted from point <m>S'</m> below the mean position, then phase angle of the particle 
                    is 
                    <me>
                      \left(\omega t - \phi_{o}\right),
                    </me>
                    and if time is counted from the point when particle is just at the mean position, 
                    then phase angle of the particle is <m>\left(\omega t \right).</m> This equation can 
                    also be the combination of both or in more general in a complex form such as 
                    <me>
                      y=A \sin(\omega t + \phi_{o}) + B \cos(\omega t+ \phi_{o}) 
                    </me>
                     <me>
                      \text{or,}\quad y = Ae^{i(kt+\phi_{o})}
                     </me>
                      </p>
  </introduction>


  <subsection xml:id="subsec-shm_energy">
    <title>Energy in SHM</title>
    <p>
      Consider a vibrating spring with mass m attached to its end, then the kinetic energy 
      of the mass 
      <me>
        K=\frac{1}{2}mv^{2},
      </me>
      and potential energy stored in the spring with a displacement x is 
      <me>
        U=\frac{1}{2}kx^{2}.
      </me>
     Now since restoring force involved in spring mass system is conservative, 
     so the total mechanical energy 
     <me>
      E=K+U
     </me>
      is conserved. 
    </p>
    <figure>
      <caption></caption>
      <sidebyside widths="30% 30%">
            
          <figure xml:id="massspring">
            <caption></caption>
            <image source="massspring.png"/>
        </figure>
        <figure xml:id="SHMenergy">
          <caption></caption>
          <image source="SHMenergy.png"/>
      </figure>
      </sidebyside>
    </figure>
    <p>
      <me>
        E = \frac{1}{2}mv^{2} +  \frac{1}{2}kx^{2} = \frac{1}{2}kA^{2} =constant
      </me>
      here k is a spring constant, A is the amplitude of vibration of a spring. 
      Let the spring oscillates in vertical up and down then the solution for SHM is given by 
      <me>
        x=y=A\sin[\omega t +\phi]
      </me>
      <me>
        \text{then}\quad v =\frac{\,dy}{\,dt} =-\omega A\cos[\omega t +\phi]
      </me>
      <me>
        \text{or,}\quad E = \frac{1}{2}mv^{2} +  \frac{1}{2}ky^{2}
      </me>
      <me>
        = \frac{1}{2}m \left(-\omega A\cos[\omega t +\phi]\right)^{2}+ \frac{1}{2}k\left(A\sin[\omega t +\phi]\right)^{2}
      </me>
      <me>
        \text{or,}\quad E = \frac{1}{2}kA^{2}\left(\cos^{2}[\omega t +\phi]+\sin^{2}[\omega t +\phi]\right) = \frac{1}{2}kA^{2}
      </me>
      <m> [\because \omega^{2}=\frac{k}{m}]</m>
    From eqn. <xref ref="eqn-shm1"/>, we have -
    <me>
      v=\pm\omega\sqrt{A^{2}-y^{2}}
    </me>
    <m>\pm</m> means mass m is oscillating in up and down direction, i.e. 
    <me>
      y=\pm A/2.
    </me>
    Now 
    <me>
      v = \pm\sqrt{\frac{k}{m}}A =\pm\omega A  \quad \text{at}\quad y=0
    </me>
       </p>
  </subsection>



  </section>

